Added substitution lemma

simple/simple.v
@@ -1,86 +1,7 @@
 Require Import Coq.Program.Equality.
-
-Parameter world : Set.
-Parameter empty : world.
-Notation "∅" := empty.
-Parameter name : world -> Set.
-Parameter link : world -> world -> Set.
-Notation "α ↪ β" := (link α β) (at level 90).
-Parameter weaken : forall {α β}, α↪β -> name β.
-Coercion weaken : link >-> name.
-Parameter import : forall {α β}, α↪β -> name α -> name β.
-Parameter next' : forall α, {β:world & α↪β}.
-Definition next α : {β:world & α↪β} := existT _ (projT1 (next' α)) (projT2 (next' α)).
-Definition next_name α := projT2 (next' α).
-Parameter export : forall {α β} (y:α↪β) (n:name β), name α + unit.
-Axiom empty_is_empty : name ∅ -> False.
-
-Definition maybe {A C} (f:A -> C) (c:C) (x:A + unit) : C :=
-match x with
-| inl a => f a
-| inr _ => c
-end.
-Definition compose {A B C:Set} (f:A -> B) (g:B -> C) (a:A) : C
- := g (f a). 
-Notation "f ○ g" := (compose g f) (at level 10).
-
-Inductive tp :=
-| one : tp
-| arrow : tp -> tp -> tp
-| sum : tp -> tp -> tp.
-
+Require Import worlds.
+Require Import typing.
 Set Implicit Arguments.
-Inductive exp (α:world) : Set :=
-| tt : exp α
-| var : name α -> exp α
-| lam : forall β, α↪β -> tp -> exp β -> exp α
-| app : exp α -> exp α -> exp α
-| inl : tp -> exp α -> exp α
-| inr : tp -> exp α -> exp α
-| case : exp α -> exp α -> exp α -> exp α.
-Implicit Arguments tt [α].
-Coercion var : name >-> exp.
-
-Definition tp_ctx γ := name γ -> tp.
-
-Definition cdot {A} : name ∅ -> A :=
-fun n => match (empty_is_empty n) with end.
-Notation "·" := cdot.
-Notation "Γ ,, ( x , T )" := ((maybe Γ T) ○ (export x)) (at level 90).
-
-Reserved Notation "Γ ⊢ E ⇐ T" (at level 90).
-
-Inductive of {γ} (Γ:tp_ctx γ) : exp γ -> tp -> Prop :=
-| tt_of : Γ ⊢ tt ⇐ one
-| var_of : forall x T,
-          Γ x = T
-        (*===============================*) ->
-          Γ ⊢ x ⇐ T
-| lam_of : forall γ' (x:γ↪γ') T S M,
-          Γ,,(x,T) ⊢ M ⇐ S
-        (*===============================*) ->
-          Γ ⊢ lam x T M ⇐ arrow T S
-| app_of : forall T S M N,
-          Γ ⊢ M ⇐ arrow T S ->
-          Γ ⊢ N ⇐ T 
-        (*===============================*) ->
-          Γ ⊢ app M N ⇐ S
-| inl_of : forall T S M,
-          Γ ⊢ M ⇐ T
-        (*===============================*) ->
-          Γ ⊢ inl S M ⇐ (sum T S)
-| inr_of : forall T S M,
-          Γ ⊢ M ⇐ S
-        (*===============================*) ->
-          Γ ⊢ inr T M ⇐ (sum T S)
-| case_of : forall T S U M N P,
-          Γ ⊢ M ⇐ (sum T S) ->
-          Γ ⊢ N ⇐ (arrow T U) ->
-          Γ ⊢ P ⇐ (arrow S U)
-        (*===============================*) ->
-          Γ ⊢ case M N P ⇐ U
-where "Γ ⊢ E ⇐ T" := (@of _ Γ E T).
-
 Inductive closure : Set :=
 | clos : forall γ, exp γ -> (name γ -> closure) -> closure.
 Definition env γ := name γ -> closure.
@@ -120,15 +41,14 @@ with env_val : forall {γ}, env γ -> Prop :=
       val V -> env_val (ρ,,(x,V)).
 
 Reserved Notation "C ⇓ V" (at level 90).
-Definition X := next_name ∅.
-Definition Y := next_name (projT1 (next' ∅)).
 Inductive eval : closure -> closure -> Prop :=
 | val_eval : forall V,
           val V
         (*======*) ->
           V ⇓ V 
 | var_eval : forall γ (ρ:env γ) x V V1,
-          ρ x = V -> V ⇓ V1
+          ρ x = V ->
+          V ⇓ V1
         (*=========*) ->
           x[ρ] ⇓ V1
 | app_eval : forall γ γ' γ'' (ρ:env γ) ρ' (x:γ'↪γ'') T M N M' V1 V2,
@@ -150,7 +70,7 @@ where "C ⇓ V" := (eval C V).
 Tactic Notation "nice_inversion" hyp(H) := inversion H; subst; simpl_existTs; subst.
 Tactic Notation "nice_inversion" integer(N) := inversion N; subst; simpl_existTs; subst.
 
-Hint Constructors eval val of closure_of.
+Hint Constructors eval val closure_of.
 
 Lemma val_env_val γ (ρ:env γ) V
  (H:val (V[ρ])) : env_val ρ.
@@ -168,23 +88,18 @@ assumption.
 nice_inversion H7.
 apply IHeval. auto.
 nice_inversion H8.
-assert (M [ρ] ∷ (arrow T1 T0)).
-eauto.
-apply IHeval1 in H3.
+assert (lam x T M' [ρ'] ∷ (arrow T1 T0)); eauto.
 nice_inversion H3.
-apply IHeval3.
 nice_inversion H13.
+apply IHeval3.
 econstructor; eauto.
-intros.
 eapply env_tp_cons; eauto.
 nice_inversion H6.
-assert (V [ρ'] ∷ T0).
-eauto.
+assert (V [ρ'] ∷ T0); eauto.
 nice_inversion H1.
 eauto.
 nice_inversion H6.
-assert (V [ρ'] ∷ S).
-eauto.
+assert (V [ρ'] ∷ S); eauto.
 nice_inversion H1.
 eauto.
 Qed.
