simple/subst.v
@@ -1,0 +1,83 @@
+Require Import Coq.Program.Equality.
+Require Import worlds.
+Require Import typing.
+Set Implicit Arguments.
+
+Section rename_sect.
+Reserved Notation "[ θ ] T " (at level 90).
+
+Fixpoint rename {α β} (θ:name α -> name β) (M:exp α) : exp β := match M with
+| var n => var (θ n)
+| tt => tt
+| app M N => app ([θ] M) ([θ] N)
+| lam _ x T M => 
+  let (_,x') := next β in
+  lam x' T ([(import x') ○ θ,,(x,x')] M)
+| inl T M => inl T ([θ] M)
+| inr T M => inr T ([θ] M)
+end
+where "[ θ ] M" := (rename θ M).
+End rename_sect.
+
+Definition import_exp {α β} (x:α↪β) : exp α -> exp β :=
+ rename (import x).
+
+Reserved Notation "[ θ ] T" (at level 90).
+Fixpoint app_subst {α β} (θ:name α -> exp β) (M:exp α) : exp β :=
+match M with
+| var n => θ n
+| tt => tt
+| app M N => app ([θ] M) ([θ] N)
+| lam _ x T M => 
+  let (β',x') := next β in
+  lam x' T ([(import_exp x') ○ θ,,(x,x')] M)
+| inl T M => inl T ([θ] M)
+| inr T M => inr T ([θ] M)
+end
+where "[ θ ] M" := (app_subst θ M).
+
+Lemma rename_lemma : forall {δ} M T (Δ:tp_ctx δ),
+  Δ ⊢ M ⇐ T ->
+  forall {γ} θ (Γ:tp_ctx γ), (forall x, Γ (θ x) = Δ x)
+(*====================================================*) ->
+  Γ ⊢ rename θ M ⇐ T. 
+induction 1; simpl; intros; subst; eauto.
+econstructor.
+set (next_link γ0).
+eapply IHof.
+intros.
+unfold compose.
+case (export x x0); simpl; intros.
+erewrite export_import_inv.
+simpl. eauto.
+erewrite export_self.
+reflexivity.
+Qed.
+
+Notation "Γ ⊩ θ ⇐ Δ" := (forall x, Γ ⊢ θ x ⇐ Δ x) (at level 90).
+
+Lemma subst_lemma : forall {δ} M T (Δ:tp_ctx δ),
+   Δ ⊢ M ⇐ T   ->
+   forall {γ} θ (Γ:tp_ctx γ), Γ ⊩ θ ⇐ Δ 
+ (*=====================================*) ->
+   Γ ⊢ [θ]M ⇐ T.
+induction 1; simpl; intros; subst; eauto.
+set (next_link γ0).
+econstructor.
+eapply IHof.
+intro.
+unfold import_exp.
+unfold compose.
+remember (export x x0).
+destruct s.
+simpl.
+specialize (H0 n).
+eapply rename_lemma.
+eassumption.
+intros. erewrite export_import_inv.
+reflexivity.
+econstructor.
+erewrite export_self.
+reflexivity.
+Qed.
+
