simple/typing.v
@@ -1,0 +1,47 @@
+Require Import worlds.
+
+Inductive tp :=
+| one : tp
+| arrow : tp -> tp -> tp
+| sum : tp -> tp -> tp.
+
+Set Implicit Arguments.
+Inductive exp (α:world) : Set :=
+| tt : exp α
+| var : name α -> exp α
+| lam : forall β, α↪β -> tp -> exp β -> exp α
+| app : exp α -> exp α -> exp α
+| inl : tp -> exp α -> exp α
+| inr : tp -> exp α -> exp α.
+Implicit Arguments tt [α].
+Coercion var : name >-> exp.
+
+Definition tp_ctx γ := name γ -> tp.
+
+Reserved Notation "Γ ⊢ E ⇐ T" (at level 90).
+
+Inductive of {γ} (Γ:tp_ctx γ) : exp γ -> tp -> Prop :=
+| tt_of : Γ ⊢ tt ⇐ one
+| var_of : forall x T,
+          Γ x = T
+        (*===============================*) ->
+          Γ ⊢ x ⇐ T
+| lam_of : forall γ' (x:γ↪γ') T S M,
+          Γ,,(x,T) ⊢ M ⇐ S
+        (*===============================*) ->
+          Γ ⊢ lam x T M ⇐ arrow T S
+| app_of : forall T S M N,
+          Γ ⊢ M ⇐ arrow T S ->
+          Γ ⊢ N ⇐ T 
+        (*===============================*) ->
+          Γ ⊢ app M N ⇐ S
+| inl_of : forall T S M,
+          Γ ⊢ M ⇐ T
+        (*===============================*) ->
+          Γ ⊢ inl S M ⇐ (sum T S)
+| inr_of : forall T S M,
+          Γ ⊢ M ⇐ S
+        (*===============================*) ->
+          Γ ⊢ inr T M ⇐ (sum T S)
+where "Γ ⊢ E ⇐ T" := (@of _ Γ E T).
+Hint Constructors of.
