simple/worlds.v
@@ -1,0 +1,34 @@
+
+Parameter world : Set.
+Parameter empty : world.
+Notation "∅" := empty.
+Parameter name : world -> Set.
+Parameter link : world -> world -> Set.
+Notation "α ↪ β" := (link α β) (at level 90).
+Parameter weaken : forall {α β}, α↪β -> name β.
+Coercion weaken : link >-> name.
+Parameter import : forall {α β}, α↪β -> name α -> name β.
+Parameter next_world : world -> world.
+Parameter next_link : forall α, α↪(next_world α).
+Definition next α : {β:world & α↪β}. 
+exists (next_world α).
+apply next_link.
+Defined.
+Parameter export : forall {α β} (y:α↪β) (n:name β), name α + unit.
+Axiom empty_is_empty : name ∅ -> False.
+Axiom export_self : forall {α β} (y:α↪β), export y y = inr _ tt.
+Axiom export_import_inv : forall {α β} (y:α↪β) x, export y (import y x) = inl _ x.
+
+Definition maybe {A C} (f:A -> C) (c:C) (x:A + unit) : C :=
+match x with
+| inl a => f a
+| inr _ => c
+end.
+Definition compose {A B C:Set} (f:A -> B) (g:B -> C) (a:A) : C
+ := g (f a). 
+Notation "f ○ g" := (compose g f) (at level 10).
+
+Definition cdot {A} : name ∅ -> A :=
+fun n => match (empty_is_empty n) with end.
+Notation "·" := cdot.
+Notation "Γ ,, ( x , T )" := ((maybe Γ T) ○ (export x)) (at level 90).
